Moved common part of wp_* lemmas' files into heap_lang_defs

fairness/heap_lang/heap_lang_defs.v
@@ -3,6 +3,7 @@ From trillium.program_logic Require Export weakestpre.
 (* From trillium.fairness Require Export resources fuel. *)
 From trillium.fairness.heap_lang Require Export lang.
 From trillium.fairness Require Export execution_model.
+From trillium.fairness.heap_lang Require Import tactics notation.
 
 (* TODO: the missing fact of em_GS etc. being typeclasses
    hardens automatic resolution of their instances *)
@@ -133,3 +134,169 @@ Section GeneralProperties.
   Proof. apply locales_of_list_from_indexes. Qed.
 
 End GeneralProperties.
+
+(** Override the notations so that scopes and coercions work out *)
+Notation "l ↦{ q } v" := (mapsto (L:=loc) (V:=val) l (DfracOwn q) v%V)
+  (at level 20, q at level 50, format "l  ↦{ q }  v") : bi_scope.
+Notation "l ↦ v" :=
+  (mapsto (L:=loc) (V:=val) l (DfracOwn 1) v%V) (at level 20) : bi_scope.
+Notation "l ↦{ q } -" := (∃ v, l ↦{q} v)%I
+  (at level 20, q at level 50, format "l  ↦{ q }  -") : bi_scope.
+Notation "l ↦ -" := (l ↦{1} -)%I (at level 20) : bi_scope.
+
+(** The tactic [inv_head_step] performs inversion on hypotheses of the shape
+[head_step]. The tactic will discharge head-reductions starting from values, and
+simplifies hypothesis related to conversions from and to values, and finite map
+operations. This tactic is slightly ad-hoc and tuned for proving our lifting
+lemmas. *)
+Ltac inv_head_step :=
+  repeat match goal with
+  | _ => progress simplify_map_eq/= (* simplify memory stuff *)
+  | H : to_val _ = Some _ |- _ => apply of_to_val in H
+  | H : head_step ?e _ _ _ _ |- _ =>
+     try (is_var e; fail 1); (* inversion yields many goals if [e] is a variable
+     and can thus better be avoided. *)
+     inversion H; subst; clear H
+  end.
+
+Local Hint Extern 0 (head_reducible _ _) => eexists _, _, _; simpl : core.
+(* Local Hint Extern 0 (head_reducible_no_obs _ _) => eexists _, _, _; simpl : core. *)
+
+(* [simpl apply] is too stupid, so we need extern hints here. *)
+Local Hint Extern 1 (head_step _ _ _ _ _) => econstructor : core.
+Local Hint Extern 0 (head_step (CmpXchg _ _ _) _ _ _ _) => eapply CmpXchgS : core.
+Local Hint Extern 0 (head_step (AllocN _ _) _ _ _ _) => apply alloc_fresh : core.
+Local Hint Resolve to_of_val : core.
+
+#[global] Instance into_val_val v : IntoVal (Val v) v.
+Proof. done. Qed.
+#[global] Instance as_val_val v : AsVal (Val v).
+Proof. by eexists. Qed.
+
+Local Ltac solve_atomic :=
+  apply strongly_atomic_atomic, ectx_language_atomic;
+    [inversion 1; naive_solver
+    |apply ectxi_language_sub_redexes_are_values; intros [] **; naive_solver].
+
+#[global] Instance rec_atomic s f x e : Atomic s (Rec f x e).
+Proof. solve_atomic. Qed.
+#[global] Instance pair_atomic s v1 v2 : Atomic s (Pair (Val v1) (Val v2)).
+Proof. solve_atomic. Qed.
+#[global] Instance injl_atomic s v : Atomic s (InjL (Val v)).
+Proof. solve_atomic. Qed.
+#[global] Instance injr_atomic s v : Atomic s (InjR (Val v)).
+Proof. solve_atomic. Qed.
+(** The instance below is a more general version of [Skip] *)
+#[global] Instance beta_atomic s f x v1 v2 : Atomic s (App (RecV f x (Val v1)) (Val v2)).
+Proof. destruct f, x; solve_atomic. Qed.
+#[global] Instance unop_atomic s op v : Atomic s (UnOp op (Val v)).
+Proof. solve_atomic. Qed.
+#[global] Instance binop_atomic s op v1 v2 : Atomic s (BinOp op (Val v1) (Val v2)).
+Proof. solve_atomic. Qed.
+#[global] Instance if_true_atomic s v1 e2 : Atomic s (If (Val $ LitV $ LitBool true) (Val v1) e2).
+Proof. solve_atomic. Qed.
+#[global] Instance if_false_atomic s e1 v2 : Atomic s (If (Val $ LitV $ LitBool false) e1 (Val v2)).
+Proof. solve_atomic. Qed.
+#[global] Instance fst_atomic s v : Atomic s (Fst (Val v)).
+Proof. solve_atomic. Qed.
+#[global] Instance snd_atomic s v : Atomic s (Snd (Val v)).
+Proof. solve_atomic. Qed.
+
+#[global] Instance fork_atomic s e : Atomic s (Fork e).
+Proof. solve_atomic. Qed.
+
+#[global] Instance alloc_atomic s v w : Atomic s (AllocN (Val v) (Val w)).
+Proof. solve_atomic. Qed.
+#[global] Instance load_atomic s v : Atomic s (Load (Val v)).
+Proof. solve_atomic. Qed.
+#[global] Instance store_atomic s v1 v2 : Atomic s (Store (Val v1) (Val v2)).
+Proof. solve_atomic. Qed.
+#[global] Instance cmpxchg_atomic s v0 v1 v2 : Atomic s (CmpXchg (Val v0) (Val v1) (Val v2)).
+Proof. solve_atomic. Qed.
+#[global] Instance faa_atomic s v1 v2 : Atomic s (FAA (Val v1) (Val v2)).
+Proof. solve_atomic. Qed.
+
+Local Ltac solve_exec_safe := intros; subst; do 3 eexists; econstructor; eauto.
+Local Ltac solve_exec_puredet := simpl; intros; by inv_head_step.
+Local Ltac solve_pure_exec :=
+  subst; intros ?; apply nsteps_once, pure_head_step_pure_step;
+    constructor; [solve_exec_safe | solve_exec_puredet].
+
+(** The behavior of the various [wp_] tactics with regard to lambda differs in
+the following way:
+
+- [wp_pures] does *not* reduce lambdas/recs that are hidden behind a definition.
+- [wp_rec] and [wp_lam] reduce lambdas/recs that are hidden behind a definition.
+
+To realize this behavior, we define the class [AsRecV v f x erec], which takes a
+value [v] as its input, and turns it into a [RecV f x erec] via the instance
+[AsRecV_recv : AsRecV (RecV f x e) f x e]. We register this instance via
+[Hint Extern] so that it is only used if [v] is syntactically a lambda/rec, and
+not if [v] contains a lambda/rec that is hidden behind a definition.
+
+To make sure that [wp_rec] and [wp_lam] do reduce lambdas/recs that are hidden
+behind a definition, we activate [AsRecV_recv] by hand in these tactics. *)
+Class AsRecV (v : val) (f x : binder) (erec : expr) :=
+  as_recv : v = RecV f x erec.
+#[global] Hint Mode AsRecV ! - - - : typeclass_instances.
+Definition AsRecV_recv f x e : AsRecV (RecV f x e) f x e := eq_refl.
+#[global] Hint Extern 0 (AsRecV (RecV _ _ _) _ _ _) =>
+  apply AsRecV_recv : typeclass_instances.
+
+#[global] Instance pure_recc f x (erec : expr) :
+  PureExec True 1 (Rec f x erec) (Val $ RecV f x erec).
+Proof. solve_pure_exec. Qed.
+#[global] Instance pure_pairc (v1 v2 : val) :
+  PureExec True 1 (Pair (Val v1) (Val v2)) (Val $ PairV v1 v2).
+Proof. solve_pure_exec. Qed.
+#[global] Instance pure_injlc (v : val) :
+  PureExec True 1 (InjL $ Val v) (Val $ InjLV v).
+Proof. solve_pure_exec. Qed.
+#[global] Instance pure_injrc (v : val) :
+  PureExec True 1 (InjR $ Val v) (Val $ InjRV v).
+Proof. solve_pure_exec. Qed.
+
+#[global] Instance pure_beta f x (erec : expr) (v1 v2 : val) `{!AsRecV v1 f x erec} :
+  PureExec True 1 (App (Val v1) (Val v2)) (subst' x v2 (subst' f v1 erec)).
+Proof. unfold AsRecV in *. solve_pure_exec. Qed.
+
+#[global] Instance pure_unop op v v' :
+  PureExec (un_op_eval op v = Some v') 1 (UnOp op (Val v)) (Val v').
+Proof. solve_pure_exec. Qed.
+
+#[global] Instance pure_binop op v1 v2 v' :
+  PureExec (bin_op_eval op v1 v2 = Some v') 1 (BinOp op (Val v1) (Val v2)) (Val v') | 10.
+Proof. solve_pure_exec. Qed.
+(* Higher-priority instance for [EqOp]. *)
+#[global] Instance pure_eqop v1 v2 :
+  PureExec (vals_compare_safe v1 v2) 1
+    (BinOp EqOp (Val v1) (Val v2))
+    (Val $ LitV $ LitBool $ bool_decide (v1 = v2)) | 1.
+Proof.
+  intros Hcompare.
+  cut (bin_op_eval EqOp v1 v2 = Some $ LitV $ LitBool $ bool_decide (v1 = v2)).
+  { intros. revert Hcompare. solve_pure_exec. }
+  rewrite /bin_op_eval /= decide_True //.
+Qed.
+
+#[global] Instance pure_if_true e1 e2 : PureExec True 1 (If (Val $ LitV $ LitBool true) e1 e2) e1.
+Proof. solve_pure_exec. Qed.
+
+#[global] Instance pure_if_false e1 e2 : PureExec True 1 (If (Val $ LitV  $ LitBool false) e1 e2) e2.
+Proof. solve_pure_exec. Qed.
+
+#[global] Instance pure_fst v1 v2 :
+  PureExec True 1 (Fst (Val $ PairV v1 v2)) (Val v1).
+Proof. solve_pure_exec. Qed.
+
+#[global] Instance pure_snd v1 v2 :
+  PureExec True 1 (Snd (Val $ PairV v1 v2)) (Val v2).
+Proof. solve_pure_exec. Qed.
+
+#[global] Instance pure_case_inl v e1 e2 :
+  PureExec True 1 (Case (Val $ InjLV v) e1 e2) (App e1 (Val v)).
+Proof. solve_pure_exec. Qed.
+
+#[global] Instance pure_case_inr v e1 e2 :
+  PureExec True 1 (Case (Val $ InjRV v) e1 e2) (App e2 (Val v)).
+Proof. solve_pure_exec. Qed.
